>[!Info] Learning Objectives
>
>- Describe the Limit Laws and understand when they can be used (and, as important, when they cannot be used)
>- Use the Limit Laws to evaluate the limit of a function
>- Use the Direct Substitution Property to evaluate the limit of a polynomial or rational function
>- Evaluate the limit of a function by first performing algebraic manipulations (factoring, conjugate multiplication, combining fractions, etc.)
>- Evaluate the limit of a function involving absolute values using the definition of an absolute value function
>- Evaluate the limit of a function by using the Squeeze Theorem, when appropriate

In this section, we establish laws for calculating limits and learn how to apply these laws. We begin by restating two useful limit results from the previous section. These two results, together with the Limit Laws, serve as a foundation for calculating many limits.

## Evaluating Finite Limits with the Limit Laws
---

We now take a look at the **Limit Laws**, the individual properties of limits. Proofs to come later.

>[!Example]- Theorem: Limit Laws
>
>Let $f(x)$ and $g(x)$ be defined for all $x\not=a$ over some open interval containing $a$. Assume that $L$ and $M$ are real numbers such that $\lim\limits_{x\to a}f(x)=L$ and $\lim\limits_{x\to a}g(x)=M$. Let $c$ be a constant. Then, each of the following holds:
>
>- **Sum Law for Limits:** $$\lim_{x\to a}(f(x)+g(x))=\lim_{x\to a}f(x)+\lim_{x\to a}g(x)=L+M$$
>- **Difference Law for Limits:** $$\lim_{x\to a}(f(x)-g(x))=\lim_{x\to a}f(x)-\lim_{x\to a}g(x)=L-M$$
>- **Constant Multiple Law for Limits:** $$\lim_{x\to a}cf(x)=c \cdot\lim_{x\to a}f(x)=cL$$
>- **Product Law for Limits:** $$\lim_{x\to a}(f(x)\cdot g(x))=\lim_{x\to a}f(x)\cdot \lim_{x\to a}g(x)=L\cdot M$$
>- **Quotient Law for Limits:** $$\lim_{x\to a}\dfrac{f(x)}{g(x)}=\dfrac{\lim\limits_{x\to a}f(x)}{\lim\limits_{x\to a}g(x)}=\dfrac{L}{M}$$ for $M\not=0$
>- **Power Law for Limits:** $$\lim_{x\to a}(f(x))^n=(\lim_{x\to a}f(x))^n=L^n$$ for every positive integer $n$
>- **Root Law for Limits:** $$\lim_{x\to a}\sqrt[n]{f(x)}=\sqrt[n]{\lim_{x\to a}f(x)}=\sqrt[n]{L}$$ for all $L$ if $n$ is odd and for $L\ge0$ if $n$ is even

>[!Danger]- Caution: The Limit Laws Require Limits to Exist
>
>A common mistake is to think that the Limit Laws apply to every limit you encounter. To be able to use the Limit Laws, both of the component limits $$\lim_{x\to a}f(x), lim_{x\to a}g(x)$$ **must** exist and be **finite**.

The following two Limit Laws together with the other Limit Laws, allow us to evaluate the limits of many algebraic functions.

>[!Example] Corollary: Basic Limit Laws
>
>For any real number $a$ and any constant $c$,
>
>1. $\lim\limits_{x\to a}x=a$
>2. $\lim\limits_{x\to a}c=c$

- Example:
	- Evaluate $\lim\limits_{x\to2}x = 2$
		- The limit of $x$ as $x$ approaches $a$ is $a$
	- Evaluate $\lim\limits_{x\to2}5 = 5$
		- The limit of a constant is that constant
	- Evaluate $\lim\limits_{x\to-3}(4x+2)$
		- $=\lim\limits_{x\to -3}(4x+2)$
		- $=\lim\limits_{x\to-3}4x+\lim\limits_{x\to -3}2$
		- $=4\lim\limits_{x\to -3}x+\lim\limits_{x\to -3}2$
		- $=4 (-3) + 2$
		- $=-10$
	- Evaluate $\lim\limits_{x\to 2}\dfrac{2x^2-3x+1}{x^3+4}$
		- $=\dfrac{\lim\limits_{x\to 2}(2x^2-3x+1)}{\lim\limits_{x\to 2}(x^3+4)}$
		- $=\dfrac{\lim\limits_{x\to2}2x^2-\lim\limits_{x\to2}3x+\lim\limits_{x\to2}1}{\lim\limits_{x\to2}x^3+\lim\limits_{x\to2}4}$
		- $=\dfrac{2 \lim\limits_{x\to2}x^2-3 \lim\limits_{x\to2}x + \lim\limits_{x\to2}1}{\lim\limits_{x\to2}x^3+\lim\limits_{x\to2}4}$
		- $=\dfrac{2(2)^2-(3\cdot2)+1}{(2)^3+4}$
		- $=\dfrac{8-6+1}{8+4}$
		- $=\dfrac{3}{12}=\dfrac{1}{4}$

## Limits of Polynomial and Rational Functions
---

>[!Example] Theorem: Direct Substitution Property (for polynomial and rational functions)
>
>Let $p(x)$ and $q(x)$ be polynomial functions. Let $a$ be a real number, then $$\lim_{x\to a}p(x)=p(a)$$ and $$\lim_{x\to a}\dfrac{p(x)}{q(x)}=\dfrac{p(a)}{q(a)}$$ when $q(a)\not= 0$
>
>**Proof**
>Let $$p(x)=c_nx^n + c_{n-1}x^{n-1} + ...+ c_1x+c_0$$
>
>Then by applying the sum, Constant Multiple, and Power Laws, we end up with $$lim_{x\to a}p(x)=\lim_{x\to a}(c_nx^n+c_{n-1}x^{n-1}+...+c_1x+c_0)$$
>$$=\lim_{x\to a}(c_nx^n)+\lim_{x\to a}(c_{n-1}x^{n-1})+...+\lim_{x\to a}(c_1x)+\lim_{x\to a}c_0$$
>$$=c_n\lim_{x\to a}x^n+c_{n-1}\lim_{x\to a}x^{n-1}+...+c_1\lim_{x\to a}x+c_0$$
>$$=c_na^n+c_{n-1}a^{n-1}+...+c_1a+c_0$$
>$$=p(a)$$
>It now follows from the Quotient Law that if $p(x)$ and $q(x)$ are polynomials for which $q(a)\not=0$ then: $$\lim_{x\to a}\dfrac{p(x)}{q(x)}=\dfrac{p(a)}{q(a)}$$

>[!Danger] Caution
>
>**Question:** Evaluate $\lim\limits_{x\to a}\dfrac{p(x)}{q(x)}$ where $\lim\limits_{x\to a}q(x)=0$
>**Student Answer:** $\dfrac{p(a)}{0}=DNE$
>**Mistake:** The Direct Substitution Property (for all rational functions) can only be applied if the limit in the denominator **is nonzero**. In fact, your answer will only be "DNE" if you have evaluated both left- and right-hand limits and found them to not be equal.

## Additional Limit Evaluation Techniques
---

We may be able to evaluate the limits of polynomials and limits of some (but not all) rational functions using the Direct Substitution Property (for polynomial and rational functions). It is possible though for $\lim\limits_{x\to a}f(x)$ to exist when $f(a)$ is undefined.

>[!Example] Theorem: Locally Equivalent Functions Have Equivalent Limits
>
>If for all $x\not=a$, $f(x)=g(x)$ over some open interval containing $a$, then: $$\lim\limits_{x\to a}f(x) = \lim\limits_{x\to a}g(x)$$ provided these limits exist.
>
>Basically we're saying that if $f(x)=g(x)$ within a given interval $(x_1, x_2)$ AND they both move toward the value $a$ (which is within the given interval $x_1<a<x_2$) then the limit as $x\to a$ for $f(x)$ will EQUAL the limit as $x\to a$ for $g(x)$.
>**Why?** Because we're saying that for all $x$ values within a given interval, $f(x)=g(x)$. If, within that interval, there is a value $a$ that $x$ approaches, both $f(x)$ and $g(x)$ will also approach the value that $a$ produces when used as an input for either/both $f(a), g(a)$. It is already established that $f(x)=g(x)$ in the interval.

Why does this matter? Because of the following example: $\lim\limits_{x\to 1}\dfrac{x^2-1}{x-1}$.

We see that $\lim\limits_{x\to 1}\dfrac{x^2-1}{x-1}=\lim\limits_{x\to 1}\dfrac{(x-1)(x+1)}{x-1}=\lim\limits_{x\to 1}(x+1)=2$. The limit has the form $\lim\limits_{x\to a}\dfrac{f(x)}{g(x)}$, where $\lim\limits_{x\to a}f(x)=0$ and $\lim\limits_{x\to a}g(x)=0$ -- $f(x)/g(x)$ has the indeterminate form 0/0). In these cases, **direct substitution** happens only after the equation is reduced as much as possible using arithmetic, algebra, and trigonometry before determining the limit (using calculus).

>[!Warning] Caution: Limits Require... Limits
>
>A common mistake is to not use limit notation when working with limits. Be aware that limit notation is _incredibly_ important in calculus and must be used up to the moment that you finish evaluating the limit.

- Another example using conjugates:
	- Evaluate $\lim\limits_{t\to 0}\dfrac{\sqrt{\cosh(t)+3}-2}{\cosh(t)-1}$
		- $=\lim\limits_{t\to 0}\bigg(\dfrac{\sqrt{\cosh(t)+3}-2}{\cosh(t)-1}\cdot\dfrac{\sqrt{\cosh(t)+3}+2}{\sqrt{\cosh(t)+3}+2} \bigg)$
		- $=\lim\limits_{t\to 0}\bigg(\dfrac{\cosh(t)+3-4}{(\cosh(t)-1)\sqrt{\cosh(t)+3}+2} \bigg)$
		- $=\lim\limits_{t\to 0}\bigg(\dfrac{\cosh(t)-1}{(\cosh(t)-1)\sqrt{\cosh(t)+3}+2} \bigg)$
		- $=\lim\limits_{t\to 0}\bigg(\dfrac{\cancel{\cosh(t)-1}}{(\cancel{cosh(t)-1})\sqrt{\cosh(t)+3}+2} \bigg)$
		- $=\bigg(\dfrac{\lim\limits_{t\to 0}1}{\lim\limits_{t\to 0}\sqrt{\cosh(t)+3}+2} \bigg)$
		- $=\bigg(\dfrac{1}{\sqrt{\lim\limits_{t\to 0}\cosh(t)+\lim\limits_{t\to 0}3}+\lim\limits_{t\to 0}2}\bigg)$
		- $=\bigg(\dfrac{1}{\sqrt{1+3}+2}\bigg)$
		- $=\dfrac{1}{\sqrt{4}+2}$
		- $=\dfrac{1}{4}$
		- Notice that substitution only happened at the end

>[!Note] Note: Conjugate Multiplication and Distribution
>
>When multiplying the numerator and denominator of an expression by a conjugate (of either numerator or denominator), it is advisable to only perform distribution **on the conjugate factors.**
>
>Problems that we encounter will **likely** cancel out if we only multiply and distribute the conjugated factors.

>[!Warning] Critical Mistake!
>
>When dealing with limits that involve expressions that use absolute value ($|f(x)|$), remember that $|f(x)|$ is not necessarily equivalent to $f(x)$. 
>
>$$\begin{equation}
>|f(x)|=\left\{ \begin{array}{cl}
>f(x) & \textrm{, if }f(x)\ge0\\
>-f(x) & \textrm{, if }f(x)<0\\
>\end{array}\right.
>\end{equation}$$
>
>Knowing the piecewise definition of the absolute value function, and using it to manipulate expressions involving absolute values, is a key component of calculus. 

Revisiting one-sided limits - modifications tot eh Limit Laws allow us to apply them to one-sided limits. To apply the Limit Laws to the limit of the form $\lim\limits_{x\to a^-}h(x)$, we require $h(x)$ to be defined over an open interval $(b,a)$; for a limit of the form $\lim\limits_{x\to a^+}h(x)$, we require the function $h(x)$ to be defined over an open interval of the form $(a,c)$.

In other words - we're examining the one-sided limits based on the open intervals where the functions are valid and approach our value $a$ from the appropriate direction. In the case of $x\to a^-$ ($x$ approaches $a$ from the left), the interval **_must_** be one such that the interval starts at the value $b<a$ (where $x$ can be any number in the interval $(b, a)$). In the case of $x\to a^+$ ($x$ approaches $a$ from the right), the interval **_must_** be one such that the interval starts at the value $c>a$ (where $x$ can be any number in the interval $(a,c)$). 

## Where the Limit Laws Break
---

Limit Laws can only be applied when the component limits are finite. A **very** common mistake made early on in calculus is to think that Limit Laws can be applied to any given limit - **this is not true**.

There is a **key difference** between algebra and calculus. In algebra, we deal with **finite** values and in calculus, we deal with levels of infinity - these concepts do **not** obey the traditional rules of arithmetic. Also, we can only use the Limit Laws **if the component limits exist and are finite.**

Strategy - use arithmetic, algebra, and trig to solve as much of the expression as possible **then** apply the Limit Laws.

>[!Warning] Answers to Pay Attention To
>
>Whenever an answer in the form of $0\cdot \infty$ appears, the answer is **wrong**. Go back to the start and apply other mathematical concepts to reduce / refactor the equation before applying the Limit Laws.

## The Squeeze Theorem
---

The **Squeeze Theorem** is useful for establishing basic trigonometric limits. It also helps us evaluate very abstract and theoretical limits for functions that cannot be described using simple functions from algebra courses. The theorem allows us to calculate limits by "squeezing" a function, with a limit at point $a$ that is unknown, between two function shaving a **common known limit at $a$**.

Think of it like a sandwitch.

>[!Example] Theorem: Squeeze Theorem
>
>Let $f(x), g(x), h(x)$ be defined for all $x\not=a$ over an open interval containing $a$. If: $$f(x)\le g(x)\le h(x)$$ for all $x\not=a$ in an open interval containing $a$ and: $$\lim_{x\to a}f(x)=L=\lim_{x\to a}h(x)$$ where $L$ is a real number, then $\lim\limits_{x\to a}g(x)=L$.
>
>This sounds more complicated than the concept is. Basically the Squeeze Theorem is saying if there are two functions ($f(x), h(x)$) that 'bound' / sandwich (are on either side) of another function ($g(x)$) along some interval $(m, n)$ that contains $a$ (such that $m<a<n$), AND if the limit of $f(x)$ as $x\to a$ = $L$ AND if the limit of $h(x)$ as $x\to a$ = $L$, then the limit of $g(x)$ as $x\to a$ MUST = $L$ because $g(x)$ is 'squeezed' between $f(x)$ and $h(x)$ in the interval. 

- Squeeze Theorem example
	- Evaluate $\lim\limits_{x\to 0}(x \cos(x))$
	- Since we don't have the calculus to solve for $\lim\limits_{x\to a}\cos(x)$, we have to use the squeeze theorem. We **do** know that $-1\le \cos(x) \le 1$, so we'll use it. 
		- $-x\le x\cos(x) \le x$
		- $\lim\limits_{x\to 0}(-x) \le \lim\limits_{x\to 0}x\cos(x) \le \lim\limits_{x\to 0}x$
		- $0\le \lim\limits_{x\to 0}x \cos(x) \le 0$ -- notice the limit of the center is still there since we can't solve for it, but it has nowhere to go. It's 'squeezed' into place by the lower and upper bounds of the inequality we've set up.
		- $\lim\limits_{x\to 0}x \cos(x) = 0$ -- we haven't actually done the 'calculus' to get here, but again, this limit has nowhere to go other than 0 **by definition**.

## Limits Involving the Sine and Cosine
---

We now use the Squeeze Theorem to tackle some limits presented as a theorem here. These limits and their use will come up in the next section and chapter.

>[!Example] Theorem: Limits of Sine and Cosine
>
>$$\lim_{\theta\to 0}(\sin(\theta))=0$$
>$$\lim_{\theta\to 0}(\cos(\theta))=1$$
>
>**Proof**
>Consider $\lim\limits_{\theta\to 0}(\sin(\theta))$. In the unit circle, we see that $\sin(\theta)$ is the y-coordinate on the unit circle. The radian measure of angle $\theta$ is the length of the arc it subtends on the unit circle. Therefore $0<\theta<\dfrac{\pi}{2}$, we have $0<\sin(\theta)<\theta$ (the $y$ value - what $\sin(\theta)$ gives us in the form of $\dfrac{y}{\textrm{hypoteneuse}}$ - is somewhere between 0 and $\theta$).
>
>From the right ($0<\theta<\frac{\pi}{2}$, quadrant 1)
>$$0\le\sin(\theta)\le\theta$$
>$$\lim_{\theta\to0^+}0\le\lim_{\theta\to0^+}\sin(\theta)\le\lim_{\theta\to0^+}\theta$$
>$$0\le\lim_{\theta\to0^+}\sin{\theta}\le0$$
>$$\lim_{\theta\to0^+}\sin(\theta)=0$$
>
>From the left ($-\frac{\pi}{2}<\theta<0$, quadrant 4)
>$$\theta\le\sin(\theta)\le0$$
>$$\lim_{\theta\to0^-}\theta\le\lim_{\theta\to0^-}\sin(\theta)\le\lim_{\theta\to0^-}0$$
>$$0<\lim_{\theta\to0^-}\sin{\theta}<0$$
>$$\lim_{\theta\to0^-}\sin(\theta)=0$$
>
>Since $\lim\limits_{\theta\to 0^-}\sin(\theta)=0$ and $\lim\limits_{\theta\to 0^+}\sin(\theta)=0$, we have a limit for $\sin(\theta)$: $$\lim_{\theta\to 0}\sin(\theta)=0$$
>
>Using the identity $\cos(\theta)=\sqrt{1-\sin^2(\theta)}$ for $-\dfrac{\pi}{2}<\theta<\dfrac{\pi}{2}$, we see that $$\lim_{\theta\to0}(\cos(\theta))=\lim_{\theta\to0}\sqrt{1-\sin^2(\theta)=1}$$
>
>Since we know that $\lim\limits_{\theta\to0}\sin(\theta)=0$:
>$$\lim_{\theta\to0}\sqrt{1-\sin^2(\theta)}$$
>$$\sqrt{\lim_{\theta\to0}1-\lim_{\theta\to0}\sin^2(\theta)}$$
>$$\sqrt{1-0^2}$$
>$$\sqrt{1}=1$$
>$$\lim_{\theta\to0}\sqrt{1-\sin^2(\theta)}=1$$
>$$\lim_{\theta\to0}\cos(\theta)=1$$

Now two limits that play important roles in later chapters:

>[!Definition] Theorem: Limits of Rational Trigonometric Functions
>
>$$\lim_{\theta\to0}\dfrac{\sin\theta}{\theta}=1$$ and
>$$\lim_{\theta\to0}\dfrac{1-\cos\theta}{\theta}=0$$
>
>**Proof**
>
>To prove the first of these limits, we use the unit circle in Figure 2.3.7. Notice this figure adds one additional triangle from the previous proof (2.3.5). We see that the length of the side opposite angle $\theta$ in this new triangle is $\tan(\theta)$. Thus, we see that for $0<\theta<\dfrac{\pi}{2}$, we have $\sin(\theta)<\theta<\tan(\theta)$.
>
>By dividing by $\sin(\theta)$ in all parts of the inequality, we obtain: $$1<\dfrac{\theta}{\sin(\theta)}<\dfrac{1}{\cos(\theta)}$$
>Equivalently, we have: $$1>\dfrac{\sin(\theta)}{\theta}>\cos(\theta)$$
>Since $\lim\limits_{\theta\to0^+}1=1=\lim\limits_{\theta\to0^+}\cos(\theta)$, we conclude that $\lim\limits_{\theta\to0^+}\dfrac{\sin(\theta)}{\theta}=1$ by the Squeeze Theorem (see above how $\dfrac{\sin(\theta)}{\theta}$ is squeezed between 1 and $\cos(\theta)$ which also goes to 1 as $\theta\to0^+$).
>
>In the following example, we'll use the above proof to establish $\lim\limits_{\theta\to0}\dfrac{1-\cos(\theta)}{\theta}=0$

![Figure 2.3.7](/files/fig-2-3-7.png)

>[!Example] Evaluating an Important Trigonometric Limit
>
>Evaluate $\lim\limits_{\theta\to0}\dfrac{1-\cos\theta}{\theta}$
>
>First step - multiply by a conjugate so we can get to $\lim\limits_{\theta\to0}\sin\theta$ since we know that.
>$$\lim_{\theta\to0}\dfrac{1-\cos\theta}{\theta} = \lim_{\theta\to0} \dfrac{1-\cos\theta}{\theta} \cdot \dfrac{1+\cos\theta}{1+\cos\theta}$$
>$$=\lim_{\theta\to0}\dfrac{1-\cos^2(\theta)}{\theta(1+\cos\theta)}$$
>$$=\lim_{\theta\to0}\dfrac{\sin^2(\theta)}{\theta(1+\cos\theta)}$$
>$$=\lim_{\theta\to0}\dfrac{\sin\theta}{\theta} \cdot\dfrac{\sin\theta}{1+\cos\theta}$$
>$$=\bigg(\lim_{\theta\to0}\dfrac{\sin\theta}{\theta}\bigg)\cdot \bigg(\lim_{\theta\to0}\dfrac{\sin\theta}{1+cos\theta}\bigg)$$
>Pulling in identities: $$\lim_{\theta\to0}\dfrac{\sin\theta}{\theta}=1, \lim_{\theta\to0}\sin\theta=0, \lim_{\theta\to0}\cos\theta=1$$
>$$=1\cdot\dfrac{0}{2}=0$$
>Therefore: $$\lim_{\theta\to0}\dfrac{1-\cos\theta}{\theta}=0$$


