
>[!Info] Learning Objectives
>
>- Compute the derivatives of the standard trigonometric functions
>- Calculate the higher-order derivatives of the sine and cosine

Simple harmonic motions (oscillations of a particle) can be described by using either sine or cosine functions. In this section we expand our knowledge of derivatives to include derivatives of trig functions. Beginning with the sine and cosine functions, we will then use them to find the derivatives of the remaining four trig functions.

## Derivatives of the Sine and Cosine Functions
---

Using the definition of a derivative, we get a practical understanding of the derivative of $/sin(x)$
- $f'(x)=\lim\limits_{h\to0}\dfrac{f(x+h)-f(x)}{h}$
- $f'(x)\approx \dfrac{f(x+h)-f(x)}{h}$ -- for values of h that are very close to 0
- $\dfrac{d}{dx}(\sin(x))\approx\dfrac{\sin(x+0.01)-\sin(x)}{0.01}$ -- substituting 0.01 for h
- $D(x)=\dfrac{\sin(x+0.01)-\sin(x)}{0.01}$
- Graphing the above function will give us a graph that's very close to the graph of the cosine function. Following the same steps to approximate the derivative of the cosine function, we'll get the negative sine function.

>[!Example] Theorem: The Derivatives of $\sin(x)$ and $\cos(x)$
>
>The derivative of the sine function is the cosine and the derivative of the cosine function is the negative sine. $$\dfrac{d}{dx}(\sin(x))=\cos(x)$$ and $$\dfrac{d}{dx}(\cos(x))=-\sin(x)$$
>
>**Proof**
>Before beginning, recall two important trigonometric limits: $$\lim_{h\to0}\dfrac{\sin(h)}{h}=1 \text{ and } \lim_{h\to0}\dfrac{\cos(h)-1}{h}=0$$
>
>Recall also the trig identity for the sine of the sum of two angles: $$\sin(x+h)=\sin(x)\cos(h) + \cos(x)\sin(h)$$
>
>Now that we have all the necessary equations and identities, we proceed with the proof
>- $\dfrac{d}{dx}(\sin(x))=\lim\limits_{h\to 0}\dfrac{\sin(x+h)-\sin(x)}{h}$
>- $=\lim\limits_{h\to0} \dfrac{\sin(x)\cos(h)+\cos(x)\sin(h)-\sin(x)}{h}$
>- $=\lim\limits_{h\to0}\bigg(\dfrac{\sin(x)\cos(h)-\sin(x)}{h}+\dfrac{\cos(x)\sin(h)}{h}\bigg)$
>- $=\lim\limits_{h\to0}\bigg(\sin(x)\bigg(\dfrac{cos(h)-1}{h}\bigg)+(\cos(x))\bigg(\dfrac{\sin(h)}{h}\bigg)\bigg)$
>- $=(\sin(x))\lim\limits_{h\to0}\bigg(\dfrac{\cos(h)-1)}{h}\bigg) + (\cos(x))\lim\limits_{h\to0} \bigg(\dfrac{\sin(h)}{h}\bigg)$
>- $=(\sin(x))(0)+(\cos(x))(1)$
>- $=\cos(x)$
>- Q.E.D.

The figure below shows the relationship between the graph of $f(x)=\sin(x)$ and its derivative $f'(x)=\cos(x)$. Notice that at the points where $f(x)=\sin(x)$ has a horizontal tangent, its derivative $f'(x)=\cos(x)$ takes on the value zero. We also see that where $f(x)=\sin(x)$ is increasing, $f'(x)=\cos(x) > 0$ and where $f(x)=\sin(x)$ is decreasing $f'(x)=\cos(x)<0$

![[fig-3-3-3.png]]

Examples!

>[!Success] Example: Differentiating a Function Containing $\sin(x)$
>
>Find the derivative of $f(x)=5x^3\sin(x)$
>- Product Rule, trig rule
>- $f'(x)g(x)+g'(x)f(x)$
>- $15x^2\sin(x)+\cos(x)5x^3$
>
>Find the derivative of $f(x)=\sin(x)\cos(x)$
>- $g(x) = \sin(x), g'(x) = \cos(x), h(x) = \cos(x), h'(x) = -\sin(x)$
>	- $f'(x)g(x) + g(x)f'(x)$
>	- $\cos(x)\cos(x) + (-\sin(x))(\sin(x))$
>	- $\cos^2(x)-\sin^2(x)$

## Derivatives of Other Trigonometric Functions
---

The remaining four trig functions may be expressed as quotients involving sine, cosine, or both. We can use the Quotient Rule to find formulas for the derivative

>[!Success] Example: The Derivative of the Tangent Function
>
>Find the derivative of $f(x)=\tan(x)$
>- $f(x)=\tan(x)=\dfrac{\sin(x)}{\cos(x)}$
>- $f'(x)=\dfrac{\cos(x)\cos(x)-(-\sin(x))(\sin(x))}{\cos^2(x)}$
>- $=\dfrac{\cos^2(x)+\sin^2(x)}{\cos^(x)}$
>- $=\dfrac{1}{\cos^2(x)}$
>- $=sec^2(x)$
>
>Find the derivative of $f(x)=\cot(x)$
>- $f(x)=\cot(x)=\dfrac{\cos(x)}{\sin(x)}$
>- $f'(x)=\dfrac{-\sin(x)\sin(x)-(\cos(x))(\cos(x))}{\sin^2(x)}$
>- $f'(x)=\dfrac{-\sin^2(x)-\cos^2(x)}{\sin^2(x)}$
>- $f'(x)=\dfrac{-1}{\sin^2(x)}$
>- $f'(x)=-\csc^2(x)$

Theroem for the derivative of all six trig functions

>[!Example] Theorem: Deriatives of $\tan(x), \cot(x), \sec(x), \csc(x)$
>
>$$\dfrac{d}{dx}(\sin(x)) = \cos(x) \qquad \dfrac{d}{dx}(\csc(x))=-\csc(x)\cot(x)$$
>$$\dfrac{d}{dx}(\cos(x))=-\sin(x) \qquad \dfrac{d}{dx}(\sec(x))=\sec(x)\tan(x)$$
>$$\dfrac{d}{dx}(\tan(x))=\sec^2(x) \qquad \dfrac{d}{dx}(\cot(x))=-\csc^2(x)$$

#practice Need to practice and review trig identities, will be important for the homework and test for this chapter, will also need to memorize the derivatives of the trig functions


